Checkpoint: experimental changes down to Mach
Propagate simple register invalidation down to Stackingproof and Mach,
where the remaining interesting changes need to be made. Elsewhere,
proofs line up and are missing at most small easy invariants.

backend/Allocproof.v
@@ -1368,21 +1368,6 @@ Qed.
 (* Definition agree_callee_save_ext (ls1 ls2: Locmap.t) (callee_sig: signature) : Prop := *)
 (*   forall l, callee_save_loc_ext l callee_sig -> ls1 l = ls2 l. *)
 
-(* TODO: Relocate "external" calling convention *)
-
-(* No registers are callee save in the external case (we would turn all
-   non-signature registers into caller-save, but registers for arguments and
-   return values are always caller-save already -- TODO establish formally for
-   the calling convention *)
-Definition callee_save_loc_ext (l: loc) :=
-  match l with
-  | R r => False
-  | S sl ofs ty => sl <> Outgoing
-  end.
-
-Definition agree_callee_save_ext (ls1 ls2: Locmap.t) : Prop :=
-  forall l, callee_save_loc_ext l -> ls1 l = ls2 l.
-
 Lemma return_regs_agree_callee_save_ext:
   forall caller callee,
   agree_callee_save_ext caller (return_regs caller callee).
