backend/LTL.v
@@ -158,6 +158,21 @@ Definition undef_caller_save_regs (ls: locset) : locset :=
     | S sl ofs ty => ls (S sl ofs ty)
     end.
 
+(* TODO: Relocate "external" calling convention *)
+
+(* No registers are callee save in the external case (we would turn all
+   non-signature registers into caller-save, but registers for arguments and
+   return values are always caller-save already -- TODO establish formally for
+   the calling convention *)
+Definition callee_save_loc_ext (l: loc) :=
+  match l with
+  | R r => False
+  | S sl ofs ty => sl <> Outgoing
+  end.
+
+Definition agree_callee_save_ext (ls1 ls2: Locmap.t) : Prop :=
+  forall l, callee_save_loc_ext l -> ls1 l = ls2 l.
+
 (** LTL execution states. *)
 
 Inductive stackframe : Type :=
