backend/Lineartyping.v
@@ -284,13 +284,13 @@ Inductive wt_state: state -> Prop :=
         (WTSTK: wt_callstack s)
         (WTFD: wt_fundef fd)
         (WTRS: wt_locset rs)
-        (AGCS: agree_callee_save rs (parent_locset s))
+        (AGCS: agree_callee_save_ext rs (parent_locset s))
         (AGARGS: agree_outgoing_arguments (funsig fd) rs (parent_locset s)),
       wt_state (Callstate s fd rs m)
   | wt_return_state: forall s rs m
         (WTSTK: wt_callstack s)
         (WTRS: wt_locset rs)
-        (AGCS: agree_callee_save rs (parent_locset s))
+        (AGCS: agree_callee_save_ext rs (parent_locset s))
         (UOUT: outgoing_undef rs),
       wt_state (Returnstate s rs m).
 
@@ -370,7 +370,8 @@ Local Opaque mreg_type.
   econstructor; eauto.
   eapply wt_find_function; eauto.
   apply wt_return_regs; auto. apply wt_parent_locset; auto.
-  red; simpl; intros. destruct l; simpl in *. rewrite H4; auto. destruct sl; auto; congruence.
+  (* red; simpl; intros. destruct l; simpl in *. rewrite H4; auto. destruct sl; auto; congruence. *)
+  red; simpl; intros. destruct l; simpl in *. contradiction. destruct sl; auto; congruence.
   red; simpl; intros. apply zero_size_arguments_tailcall_possible in H. apply H in H4. contradiction.
 - (* builtin *)
   simpl in *; InvBooleans.
@@ -392,48 +393,50 @@ Local Opaque mreg_type.
   apply wt_undef_regs; auto.
 - (* return *)
   simpl in *. InvBooleans.
-  destruct (Genv.type_of_call ge (call_comp s) (callee_comp s)).
-  {
-  econstructor; eauto.
-  apply wt_return_regs; auto. apply wt_parent_locset; auto.
-  red; simpl; intros. destruct l; simpl in *. rewrite H0; auto. destruct sl; auto; congruence.
-  red; simpl; intros. auto.
-  }
+  (* destruct (Genv.type_of_call ge (call_comp s) (callee_comp s)). *)
+  (* { *)
+  (* econstructor; eauto. *)
+  (* apply wt_return_regs; auto. apply wt_parent_locset; auto. *)
+  (* red; simpl; intros. destruct l; simpl in *. rewrite H0; auto. destruct sl; auto; congruence. *)
+  (* red; simpl; intros. auto. *)
+  (* } *)
   { (* new case*)
-  (* econstructor; eauto. (* FIXME *) *)
-  admit.
-  }
-  { (* same as Genv.InternalCall *)
   econstructor; eauto.
-  apply wt_return_regs; auto. apply wt_parent_locset; auto.
-  red; simpl; intros. destruct l; simpl in *. rewrite H0; auto. destruct sl; auto; congruence.
+  apply wt_return_regs_ext; auto. apply wt_parent_locset; auto.
+  red; simpl; intros. destruct l; simpl in *. contradiction. destruct sl; auto; congruence.
   red; simpl; intros. auto.
   }
+  (* { (* same as Genv.InternalCall *) *)
+  (* econstructor; eauto. *)
+  (* apply wt_return_regs; auto. apply wt_parent_locset; auto. *)
+  (* red; simpl; intros. destruct l; simpl in *. rewrite H0; auto. destruct sl; auto; congruence. *)
+  (* red; simpl; intros. auto. *)
+  (* } *)
 - (* internal function *)
   simpl in WTFD.
   econstructor. eauto. eauto. eauto.
-  destruct (Genv.type_of_call ge (call_comp s) (comp_of f)).
-  {
-  apply wt_undef_regs. apply wt_call_regs. auto.
-  }
+  (* destruct (Genv.type_of_call ge (call_comp s) (comp_of f)). *)
+  (* { *)
+  (* apply wt_undef_regs. apply wt_call_regs. auto. *)
+  (* } *)
   { (* new case *)
   apply wt_undef_regs. apply wt_call_regs_ext. auto.
   }
-  { (* same as Genv.InternalCall *)
-  apply wt_undef_regs. apply wt_call_regs. auto.
-  }
+  (* { (* same as Genv.InternalCall *) *)
+  (* apply wt_undef_regs. apply wt_call_regs. auto. *)
+  (* } *)
 - (* external function *)
   econstructor. auto. apply wt_setpair. 
   eapply external_call_well_typed; eauto.
   apply wt_undef_caller_save_regs; auto.
   red; simpl; intros. destruct l; simpl in *.
-  rewrite locmap_get_set_loc_result by auto. simpl. rewrite H; auto. 
+  (* rewrite locmap_get_set_loc_result by auto. simpl. rewrite H; auto.  *)
+  contradiction.
   rewrite locmap_get_set_loc_result by auto. simpl. destruct sl; auto; congruence.
   red; simpl; intros. rewrite locmap_get_set_loc_result by auto. auto.
 - (* return *)
   inv WTSTK. econstructor; eauto.
-(* Qed. *)
-Admitted.
+Qed.
 
 Theorem wt_initial_state:
   forall S, initial_state prog S -> wt_state S.
@@ -493,7 +496,8 @@ Qed.
 Lemma wt_callstate_agree:
   forall s f rs m,
   wt_state (Callstate s f rs m) ->
-  agree_callee_save rs (parent_locset s) /\ agree_outgoing_arguments (funsig f) rs (parent_locset s).
+  (* agree_callee_save rs (parent_locset s) /\ agree_outgoing_arguments (funsig f) rs (parent_locset s). *)
+  agree_callee_save_ext rs (parent_locset s) /\ agree_outgoing_arguments (funsig f) rs (parent_locset s).
 Proof.
   intros. inv H; auto.
 Qed.
@@ -501,7 +505,8 @@ Qed.
 Lemma wt_returnstate_agree:
   forall s rs m,
   wt_state (Returnstate s rs m) ->
-  agree_callee_save rs (parent_locset s) /\ outgoing_undef rs.
+  (* agree_callee_save rs (parent_locset s) /\ outgoing_undef rs. *)
+  agree_callee_save_ext rs (parent_locset s) /\ outgoing_undef rs.
 Proof.
   intros. inv H; auto.
 Qed.
