backend/Tunnelingproof.v
@@ -678,7 +678,7 @@ Proof.
     assert (X: Genv.type_of_call ge (comp_of f) (Genv.find_comp ge vf) = Genv.CrossCompartmentCall).
     { erewrite find_comp_translated, type_of_call_translated; eauto. }
     specialize (NO_CROSS_PTR X).
-    rewrite X in NO_CROSS_PTR, EV. rewrite H1.
+    (* rewrite X in NO_CROSS_PTR, EV. rewrite H1. *)
     apply Forall_forall. rewrite Forall_forall in NO_CROSS_PTR.
     intros v Hin. apply in_map_iff in Hin as [v' [Heq Hin]].
     apply in_map with (f := (fun p : rpair loc => Locmap.getpair p (undef_regs destroyed_at_function_entry (call_regs_ext rs (funsig fd)))))
@@ -697,28 +697,33 @@ Proof.
                    (fun p : rpair loc =>
                     Locmap.getpair p
                       (undef_regs destroyed_at_function_entry
-                         match Genv.type_of_call ge (comp_of f) (Genv.find_comp ge vf) with
-                         | Genv.CrossCompartmentCall => call_regs_ext rs (funsig fd)
-                         | _ => call_regs rs
-                         end)) (Conventions.loc_parameters (funsig fd)))
+                         (* match Genv.type_of_call ge (comp_of f) (Genv.find_comp ge vf) with *)
+                         (* | Genv.CrossCompartmentCall => call_regs_ext rs (funsig fd) *)
+                         (* | _ => call_regs rs *)
+                         (* end *)
+                         (call_regs_ext rs (funsig fd))
+                   )) (Conventions.loc_parameters (funsig fd)))
                 (map
                    (fun p : rpair loc =>
                     Locmap.getpair p
                       (undef_regs destroyed_at_function_entry
-                         match Genv.type_of_call tge (comp_of (tunnel_function f)) (Genv.find_comp ge vf) with
-                         | Genv.CrossCompartmentCall => call_regs_ext tls (funsig fd)
-                         | _ => call_regs tls
-                         end)) (Conventions.loc_parameters (funsig fd)))).
+                         (* match Genv.type_of_call tge (comp_of (tunnel_function f)) (Genv.find_comp ge vf) with *)
+                         (* | Genv.CrossCompartmentCall => call_regs_ext tls (funsig fd) *)
+                         (* | _ => call_regs tls *)
+                         (* end *)
+                         (call_regs_ext tls (funsig fd))
+                   )) (Conventions.loc_parameters (funsig fd)))).
   { apply locmap_getpairs_lessdef.
     apply locmap_undef_regs_lessdef.
     assert (EQ: Genv.type_of_call ge (comp_of f) (Genv.find_comp ge vf)
                 = Genv.type_of_call tge (comp_of (tunnel_function f)) (Genv.find_comp ge vf)). {
       rewrite type_of_call_translated, find_comp_translated. reflexivity. }
-    rewrite EQ.
-    destruct (Genv.type_of_call tge (comp_of (tunnel_function f)) (Genv.find_comp ge vf)).
-    apply call_regs_lessdef. auto.
+    (* rewrite EQ. *)
+    (* destruct (Genv.type_of_call tge (comp_of (tunnel_function f)) (Genv.find_comp ge vf)). *)
+    (* apply call_regs_lessdef. auto. *)
     apply call_regs_ext_lessdef. auto.
-    apply call_regs_lessdef. auto. }
+    (* apply call_regs_lessdef. auto. *)
+  }
   rewrite <- find_comp_translated, comp_tunnel_fundef.
   eapply call_trace_lessdef; eauto using symbols_preserved, senv_preserved.
   econstructor; eauto.
@@ -787,11 +792,11 @@ Proof.
   { inv STK; [reflexivity |]. inv H0; reflexivity. }
   assert (CALLEE : callee_comp s = callee_comp ts).
   { inv STK; [reflexivity |]. inv H0; reflexivity. }
-  rewrite type_of_call_translated, CALLER, CALLEE.
-  destruct (Genv.type_of_call tge (call_comp ts) (callee_comp ts)).
-  constructor; eauto using return_regs_lessdef, match_parent_locset.
+  (* rewrite type_of_call_translated, CALLER, CALLEE. *)
+  (* destruct (Genv.type_of_call tge (call_comp ts) (callee_comp ts)). *)
+  (* constructor; eauto using return_regs_lessdef, match_parent_locset. *)
   constructor; eauto using return_regs_ext_lessdef, match_parent_locset.
-  constructor; eauto using return_regs_lessdef, match_parent_locset.
+  (* constructor; eauto using return_regs_lessdef, match_parent_locset. *)
 - (* internal function *)
   exploit Mem.alloc_extends. eauto. eauto. apply Z.le_refl. apply Z.le_refl.
   intros (tm' & ALLOC & MEM'). 
@@ -804,11 +809,11 @@ Proof.
   { inv STK; [reflexivity |]. inv H0; reflexivity. }
   assert (CALLEE : comp_of f = comp_of (tunnel_function f)).
   { reflexivity. }
-  rewrite type_of_call_translated, CALLER, CALLEE.
-  destruct (Genv.type_of_call tge (call_comp ts) (comp_of (tunnel_function f))).
-  simpl. econstructor; eauto using locmap_undef_regs_lessdef, call_regs_lessdef.
+  (* rewrite type_of_call_translated, CALLER, CALLEE. *)
+  (* destruct (Genv.type_of_call tge (call_comp ts) (comp_of (tunnel_function f))). *)
+  (* simpl. econstructor; eauto using locmap_undef_regs_lessdef, call_regs_lessdef. *)
   simpl. econstructor; eauto using locmap_undef_regs_lessdef, call_regs_ext_lessdef.
-  simpl. econstructor; eauto using locmap_undef_regs_lessdef, call_regs_lessdef.
+  (* simpl. econstructor; eauto using locmap_undef_regs_lessdef, call_regs_lessdef. *)
 - (* external function *)
   exploit external_call_mem_extends; eauto using locmap_getpairs_lessdef.
   intros (tvres & tm' & A & B & C & D).
